Working on SubMulti, through Tlet case
Now substitute with map
Semantics in terms of lists (elements, keylist, vals)
Define lists of maps, prove theorems
Prove new versions of aux lemmas for SubMulti
Did all term cases before Tmatch

proofs/common/AssocList.v
@@ -10,7 +10,7 @@ Import gmap.
 
 Section FixTypes.
 
-Context (A B: Type) `{A_eq: EqDecision A} `{A_count: Countable A}.
+Context (A B: Type) `{A_count: Countable A}.
 
 Definition amap := gmap A B. (*NOTE: we DONT want to export stdpp everywhere, so we provide our own defs*)
 
@@ -82,11 +82,17 @@ Definition amap_size (m: amap) : nat := size m.
 
 Definition amap_is_empty (m: amap) : bool := Nat.eqb (size m) 0.
 
+(*map diff - but we want to remove a subset of keys*)
+Definition amap_remove (x: A) (m: amap) := delete x m.
+
+Definition amap_diff (m: amap) (s: aset A) : amap :=
+  set_fold amap_remove m s.
+
 (*Proofs*)
 
 Ltac unfold_amap :=
   repeat (progress (unfold amap, amap_empty, amap_in, amap_lookup, amap_set, amap_replace, amap_change,
-  amap_union, amap_size, amap_is_empty, amap_singleton in *)).
+  amap_union, amap_size, amap_is_empty, amap_singleton, amap_remove, amap_diff in *)).
 Ltac simpl_amap := unfold_amap; simplify_map_eq.
 Ltac solve_amap := unfold_amap; simplify_map_eq; solve[auto].
 
@@ -179,6 +185,55 @@ Proof.
   - erewrite amap_union_notin; auto.
 Qed.
 
+Lemma amap_remove_same x m:
+  amap_lookup (amap_remove x m) x = None.
+Proof.
+  solve_amap.
+Qed.
+
+Lemma amap_remove_diff x m y:
+  x <> y ->
+  amap_lookup (amap_remove x m) y = amap_lookup m y.
+Proof.
+  intros Hxy. solve_amap.
+Qed.
+
+Lemma amap_diff_in m s x:
+  aset_mem x s ->
+  amap_lookup (amap_diff m s) x = None.
+Proof.
+  unfold amap_diff.
+  apply aset_fold_ind with (P:=fun r s => aset_mem x s -> amap_lookup r x = None).
+  - intros Hmem. simpl_set.
+  - intros y s1 b Hnotin IH Hin.
+    simpl_set. destruct (EqDecision0 x y); subst.
+    + rewrite amap_remove_same. auto.
+    + destruct Hin; [simpl_set; subst; contradiction|].
+      rewrite amap_remove_diff; auto.
+Qed.
+
+Lemma amap_diff_notin m s x:
+  ~ aset_mem x s ->
+  amap_lookup (amap_diff m s) x = amap_lookup m x.
+Proof.
+  unfold amap_diff.
+  apply aset_fold_ind with (P:=fun r s => ~ aset_mem x s -> amap_lookup r x = amap_lookup m x); auto.
+  intros y s1 b Hnotin IH Hin.
+  simpl_set. destruct (EqDecision0 x y); subst.
+  - exfalso; apply Hin; auto.
+  - rewrite amap_remove_diff; auto.
+Qed.
+
+Lemma amap_diff_lookup_impl m s x y:
+  amap_lookup (amap_diff m s) x = Some y ->
+  amap_lookup m x = Some y.
+Proof.
+  intros Hlookup.
+  destruct (aset_mem_dec x s).
+  - rewrite amap_diff_in in Hlookup; auto. discriminate.
+  - rewrite amap_diff_notin in Hlookup; auto.
+Qed.
+
 (*Lemmas about [keys]*)
 Lemma keys_empty: keys amap_empty = aset_empty.
 Proof. reflexivity. Qed.
@@ -189,7 +244,7 @@ Proof.
   set_unfold. intros x1. split.
   - intros [[x2 y2] [Hx1 Hin]].
     subst. simpl. apply elem_of_map_to_list in Hin.
-    destruct (A_eq x x2); subst; auto.
+    destruct (EqDecision0 x x2); subst; auto.
     rewrite lookup_insert_ne in Hin; auto.
     solve_amap.
   - intros Hx; subst. exists (x, y). split; auto.
@@ -235,7 +290,7 @@ Proof.
   set_unfold. intros Hnotin x1. split; unfold amap in *.
   - intros [[x2 y2] [Hx1 Hin]]; subst; simpl.
     apply elem_of_map_to_list in Hin. 
-    destruct (A_eq x x2); subst; auto.
+    destruct (EqDecision0 x x2); subst; auto.
     rewrite lookup_insert_ne in Hin by auto.
     left. exists (x2, y2). split; auto.
     apply elem_of_map_to_list. auto.
@@ -384,6 +439,123 @@ Proof.
   apply Nat.eqb_eq.
 Qed.
 
+(*Get values as list*)
+Definition elements (m: amap) : list (A * B) := map_to_list m.
+
+Lemma in_elements_iff x y (m: amap):
+  List.In (x, y) (elements m) <-> amap_lookup m x = Some y.
+Proof.
+  unfold elements, amap_lookup.
+  rewrite <- elem_of_list_In. apply elem_of_map_to_list.
+Qed.
+
+Definition keylist (m: amap) : list A := map fst (elements m).
+
+Lemma in_keylist_iff x (m: amap):
+  List.In x (keylist m) <-> amap_mem x m.
+Proof.
+  unfold keylist. rewrite in_map_iff; unfold amap_mem. split.
+  - intros [[x1 y1] [Hx Hinxy]]. subst; simpl. 
+    apply in_elements_iff in Hinxy. rewrite Hinxy; auto.
+  - destruct (amap_lookup m x) as [y|] eqn : Hlookup; try discriminate.
+    intros _. exists (x, y). split; auto; apply in_elements_iff; auto.
+Qed.
+
+Definition vals (m: amap) : list B := map snd (elements m).
+
+Definition in_vals_iff y (m: amap):
+  List.In y (vals m) <-> exists x, amap_lookup m x = Some y.
+Proof.
+  unfold vals. rewrite in_map_iff.
+  split.
+  - intros [[x1 y1] [Hy Hin]]. 
+    rewrite in_elements_iff in Hin. subst. simpl.
+    eauto.
+  - intros [x Hlookup]. exists (x, y). split; auto.
+    apply in_elements_iff. auto.
+Qed.
+
+Lemma elements_eq m: elements m = combine (keylist m) (vals m).
+Proof.
+  unfold keylist, vals. symmetry; apply combine_eq.
+Qed. 
+
+(*lengths*)
+Lemma elements_length m:
+  length (elements m) = amap_size m.
+Proof.
+  apply map_to_list_length.
+Qed.
+Lemma keylist_length m:
+  length (keylist m) = amap_size m.
+Proof.
+  unfold keylist. simpl_len. apply elements_length. 
+Qed.
+
+Lemma vals_length m:
+  length (vals m) = amap_size m.
+Proof.
+  unfold vals. simpl_len. apply elements_length.
+Qed.
+
+(*NoDup*)
+Lemma elements_Nodup m:
+  List.NoDup (elements m).
+Proof.
+  apply NoDup_ListNoDup, NoDup_map_to_list.
+Qed.
+
+Lemma keylist_Nodup m:
+  List.NoDup (keylist m).
+Proof.
+  unfold keylist. apply NoDup_ListNoDup.
+  apply NoDup_fst_map_to_list.
+Qed.
+
+(*Forall over map*)
+Definition amap_Forall (P: A -> B -> Prop) (m: amap) : Prop :=
+  map_Forall P m.
+
+Lemma amap_Forall_forall (P: A -> B -> Prop) (m: amap):
+  amap_Forall P m <-> forall x y, amap_lookup m x = Some y -> P x y.
+Proof.
+  unfold amap_Forall. apply map_Forall_lookup.
+Qed.
+
+Lemma amap_Forall_elements (P: A -> B -> Prop) (m: amap) :
+  amap_Forall P m <-> Forall2 P (keylist m) (vals m).
+Proof.
+  unfold amap_Forall. rewrite Forall2_combine.
+  assert (Hlen: length (keylist m) = length (vals m)) by (unfold keylist, vals; solve_len).
+  rewrite <- elements_eq. unfold elements.
+  split. (*have to split bc rewrite doesnt work*) 
+  - intros Hall. apply map_Forall_to_list in Hall. split; auto.
+    revert Hall. apply List.Forall_impl. intros [x y]; auto.
+  - intros [_ Hall2]. apply map_Forall_to_list. revert Hall2.
+    apply List.Forall_impl. intros [x y]; auto.
+Qed.
+  
+
+(*Get values as set - NOTE dont do because dont want countable*)
+(* Section BCount.
+
+Context `{countable.Countable B}.
+
+Definition vals (m: amap) : aset B := map_to_set (fun _ (x: B) => x) m.
+
+Lemma amap_mem_vals (y: B) (m: amap): aset_mem y (vals m) <-> exists (x: A), amap_lookup m x = Some y.
+Proof.
+  unfold amap_lookup, aset_mem, vals.
+  set_unfold.
+  split.
+  - intros [[x1 y1] [Hy Hinx]]. subst; simpl.
+    exists x1. apply elem_of_map_to_list in Hinx. auto.
+  - intros [x Hlookup]. exists (x, y). split; auto. apply elem_of_map_to_list. auto.
+Qed.
+
+End BCount. *)
+
+
 (*[get_assoc_list_nodup] is always true now*)
 (* Lemma amap_lookup_nodup
   (m: amap) (x: A) (y: B)
@@ -417,9 +589,23 @@ Qed. *)
 
 End FixTypes.
 
-Definition amap_map {A B C: Type} `{A_eq: EqDecision A} `{A_count: Countable A} 
+Definition amap_map {A B C: Type} `{A_count: Countable A} 
   (f: B -> C) (m: amap A B) : amap A C :=
   fmap f m.
+
+(*Dependent map - NOTE: this is inefficient, since we convert to a list and back*)
+(*Definition amap_dep_map {A B C: Type} {P: A -> B -> Prop} (f: forall x y, P x y -> C) (m: amap A B)
+  (Hall: amap_Forall P m) : amap A C :=
+  
+
+
+Definition dep_map {A B: Type} {P: A -> Prop} (f: forall x, P x -> B) := 
+fix dep_map (l: list A) (Hall: Forall P l) : list B :=
+  match l as l' return Forall P l' -> list B with
+  | nil => fun _ => nil
+  | x :: tl => fun Hforall => f x (Forall_inv Hforall) ::
+    dep_map tl (Forall_inv_tail Hforall)
+  end Hall. *)
 
 End Map.
 
@@ -435,6 +621,12 @@ Arguments amap_union {_} {_} {_} {_}.
 Arguments amap_mem {_} {_} {_} {_}.
 Arguments amap_size {_} {_} {_} {_}.
 Arguments amap_is_empty {_} {_} {_} {_}.
+Arguments amap_diff {_} {_} {_} {_}.
+Arguments elements {_} {_} {_} {_}.
+Arguments vals {_} {_} {_} {_}.
+Arguments keylist {_} {_} {_} {_}.
+Arguments amap_Forall {_} {_} {_} {_}.
+
 
 (*TODO: let's try this instead of lemmas maybe?*)
 From stdpp Require Import fin_maps.
